---
---
{% include math.html %}


$$
{d \over dx}(\csc (x)) = -\csc (x) \cdot \cot (x)
$$

$$
h(x) = {csc(3x) \over x^3}
$$

$$
h(x) = csc(3x) \cdot x^{-3}
$$

Product rule

$$
{d \over dx}(a\cdot b) = \dot{a}\cdot b + a \cdot \dot{b}
$$


$$ a = \csc(3x) $$

$$ b = x^{-3} $$

$$ \dot a = -3\csc (x) \cdot \cot (x) $$

$$ \dot b = -3 \cdot x^{-4} $$

$$ (-3\csc (3x) \cdot \cot (3x)) \cdot (x^{-3}) + (\csc(3x)) \cdot (-3 \cdot x^{-4}) $$

$$ -3 {\csc (3x) \cdot \cot (3x) \over x^3} + -3 {csc(3x) \over x^4}$$

$$ -3 \csc (3x) \cdot ({cot (3x) \over x^3} + {1 \over x^4}) $$


$$ -3 \csc (3x) \cdot ({cot (3x) \over x^3}\cdot{x \over x} + {1 \over x^4}) $$


